code/ecdsap256/Hacl.Impl.P.LowLevel.fst
@@ -11,7 +11,6 @@ open Hacl.Spec.P256.Definition
 open Hacl.Lemmas.P256
 
 open Spec.P256
-open Spec.ECDSA
 
 open FStar.Math
 open FStar.Math.Lemmas
@@ -19,9 +18,6 @@ open FStar.Mul
 
 open FStar.Tactics
 open FStar.Tactics.Canon
-
-(* open Spec.P256.Lemmas *)
-open Lib.IntTypes.Intrinsics
 
 open Hacl.Impl.P256.LowLevel
 open Hacl.Impl.P384.LowLevel
